code/ecdsap256/Hacl.Impl.P256.Bignum.fsti
@@ -10,6 +10,8 @@ open Lib.Buffer
 
 open Hacl.Spec.P256.Felem
 
+module BSeq = Lib.ByteSequence
+
 #set-options "--z3rlimit 50 --fuel 0 --ifuel 0"
 
 // TODO: mv
@@ -22,6 +24,7 @@ val scalar_bit:
     (requires fun h -> live h s)
     (ensures  fun h0 r h1 -> h0 == h1 /\
       r == Spec.ECDSA.ith_bit (as_seq h0 s) (v n) /\ v r <= 1)
+
 
 ///  Create a bignum
 
@@ -59,23 +62,23 @@ val bn_is_zero_vartime4: f:felem -> Stack bool
 val bn_is_zero_mask4: f:felem -> Stack uint64
   (requires fun h -> live h f)
   (ensures fun h0 r h1 -> modifies0 h0 h1 /\
-    (if as_nat h0 f = 0 then uint_v r == pow2 64 - 1 else uint_v r == 0))
+    (if as_nat h0 f = 0 then v r == ones_v U64 else v r == 0))
 
 
 val bn_is_eq_mask4: a:felem -> b:felem -> Stack uint64
   (requires fun h -> live h a /\ live h b)
   (ensures fun h0 r h1 -> modifies0 h0 h1 /\
-    (if as_nat h0 a = as_nat h0 b then uint_v r == pow2 64 - 1 else uint_v r = 0))
+    (if as_nat h0 a = as_nat h0 b then v r == ones_v U64 else v r = 0))
 
 
 ///  Conditional copy
 
 // NOTE: changed precondition `eq_or_disjoint res x`
 val bn_copy_conditional4: res:felem -> x:felem
-  -> mask:uint64{uint_v mask = 0 \/ uint_v mask = pow2 64 - 1} -> Stack unit
+  -> mask:uint64{v mask = 0 \/ v mask = ones_v U64} -> Stack unit
   (requires fun h -> live h res /\ live h x /\ eq_or_disjoint res x)
   (ensures fun h0 _ h1 -> modifies (loc res) h0 h1 /\
-    (if uint_v mask = 0 then as_seq h1 res == as_seq h0 res else as_seq h1 res == as_seq h0 x))
+    (if v mask = 0 then as_seq h1 res == as_seq h0 res else as_seq h1 res == as_seq h0 x))
 
 
 val bn_cmovznz4: cin:uint64 -> x:felem -> y:felem -> res:felem -> Stack unit
@@ -83,7 +86,7 @@ val bn_cmovznz4: cin:uint64 -> x:felem -> y:felem -> res:felem -> Stack unit
     live h x /\ live h y /\ live h res /\
     disjoint x res /\ eq_or_disjoint y res)
   (ensures fun h0 _ h1 -> modifies1 res h0 h1 /\
-    (if uint_v cin = 0 then as_nat h1 res == as_nat h0 x else as_nat h1 res == as_nat h0 y))
+    (if v cin = 0 then as_nat h1 res == as_nat h0 x else as_nat h1 res == as_nat h0 y))
 
 
 ///  Addition and subtraction
@@ -105,7 +108,7 @@ val bn_sub4: x:felem -> y:felem -> res:felem -> Stack uint64
     eq_or_disjoint x y /\ eq_or_disjoint x res /\ eq_or_disjoint y res)
   (ensures fun h0 c h1 -> modifies1 res h0 h1 /\ v c <= 1 /\
     as_nat h1 res - v c * pow2 256 == as_nat h0 x - as_nat h0 y /\
-    (if uint_v c = 0 then as_nat h0 x >= as_nat h0 y else as_nat h0 x < as_nat h0 y))
+    (if v c = 0 then as_nat h0 x >= as_nat h0 y else as_nat h0 x < as_nat h0 y))
 
 
 // TODO: rm; use sub4
@@ -115,7 +118,7 @@ val bn_sub4_il: x:felem -> y:glbuffer uint64 (size 4) -> res:felem -> Stack uint
     disjoint x res /\ disjoint res y)
   (ensures fun h0 c h1 -> modifies1 res h0 h1 /\ v c <= 1 /\
     as_nat h1 res - v c * pow2 256 == as_nat h0 x - as_nat_il h0 y /\
-    (if uint_v c = 0 then as_nat h0 x >= as_nat_il h0 y else as_nat h0 x < as_nat_il h0 y))
+    (if v c = 0 then as_nat h0 x >= as_nat_il h0 y else as_nat h0 x < as_nat_il h0 y))
 
 
 val bn_sub_mod4: x:felem -> y:felem -> n:felem -> res:felem -> Stack unit
@@ -147,7 +150,7 @@ val bn_sqr4: f:felem -> res:widefelem -> Stack unit
 
 ///  pow2-operations
 
-val bn_lshift256: f:felem -> res:lbuffer uint64 (size 8) -> Stack unit
+val bn_lshift256: f:felem -> res:lbuffer uint64 8ul -> Stack unit
   (requires fun h ->
     live h f /\ live h res /\ disjoint f res)
   (ensures fun h0 _ h1 -> modifies1 res h0 h1 /\
@@ -155,24 +158,30 @@ val bn_lshift256: f:felem -> res:lbuffer uint64 (size 8) -> Stack unit
 
 
 ///  Conversion between bignum and bytes representation
-// TODO: rm Spec.ECDSA here
 
-val bn_to_bytes_be4: f:felem -> res:lbuffer uint8 (32ul) -> Stack unit
-  (requires fun h -> live h f /\ live h res /\ disjoint f res)
+val bn_to_bytes_be4: f:felem -> res:lbuffer uint8 32ul -> Stack unit
+  (requires fun h ->
+    live h f /\ live h res /\ disjoint f res /\
+    as_nat h f < pow2 256)
   (ensures fun h0 _ h1 -> modifies (loc res) h0 h1 /\
-    as_seq h1 res == Lib.ByteSequence.uints_to_bytes_be #_ #_ #4 (as_seq h0 f))
+    as_seq h1 res == BSeq.nat_to_bytes_be 32 (as_nat h0 f))
 
 
-// TODO: rm
-inline_for_extraction noextract
-val changeEndian: i:felem -> Stack unit
-  (requires fun h -> live h i)
-  (ensures  fun h0 _ h1 -> modifies1 i h0 h1 /\
-    as_seq h1 i == Spec.ECDSA.changeEndian (as_seq h0 i) /\
-    as_nat h1 i < pow2 256)
-
-
-val bn_from_bytes_be4: b:lbuffer uint8 (size 32) -> res:felem -> Stack unit
+val bn_from_bytes_be4: b:lbuffer uint8 32ul -> res:felem -> Stack unit
   (requires fun h -> live h b /\ live h res /\ disjoint b res)
   (ensures  fun h0 _ h1 -> modifies (loc res) h0 h1 /\
-    as_seq h1 res == Spec.ECDSA.changeEndian (Lib.ByteSequence.uints_from_bytes_be (as_seq h0 b)))
+    as_nat h1 res == BSeq.nat_from_bytes_be (as_seq h0 b))
+
+
+val bn_to_bytes_le4: f:felem -> res:lbuffer uint8 32ul -> Stack unit
+  (requires fun h ->
+    live h f /\ live h res /\ disjoint f res /\
+    as_nat h f < pow2 256)
+  (ensures fun h0 _ h1 -> modifies (loc res) h0 h1 /\
+    as_seq h1 res == BSeq.nat_to_bytes_le 32 (as_nat h0 f))
+
+
+val bn_from_bytes_le4: b:lbuffer uint8 32ul -> res:felem -> Stack unit
+  (requires fun h -> live h b /\ live h res /\ disjoint b res)
+  (ensures  fun h0 _ h1 -> modifies (loc res) h0 h1 /\
+    as_nat h1 res == BSeq.nat_from_bytes_le (as_seq h0 b))
